Splinter/LikesCoordinationLayer/LikesCrashTolerantJournal.i.dfy
@@ -1,0 +1,199 @@
+include "../Journal/LikesJournal.i.dfy"
+include "../CoordinationLayer/CrashTolerantJournal.i.dfy"
+
+module LikesCrashTolerantJournal {
+  import opened Options
+  import opened GenericDisk
+  import opened LikesMod
+  import CrashTolerantJournal
+  import LinkedJournal
+  import LikesJournal
+
+  // base label InternalLabel is the only one that has allocations
+  datatype TransitionLabel = TransitionLabel(allocs: seq<Address>, base: CrashTolerantJournal.TransitionLabel)
+
+  type StoreImage = LinkedJournal.TruncatedJournal
+
+  datatype Ephemeral =
+    | Unknown  // This means None
+    | Known(v: LikesJournal.Variables)
+  {
+    predicate WF() {
+      Known? ==> v.WF()
+    }
+  }
+
+  datatype Variables = Variables(
+    persistent: StoreImage,
+    ephemeral: Ephemeral,
+    inFlight: Option<StoreImage>
+  ){
+    predicate WF() {
+      && persistent.WF()
+      && ephemeral.WF()
+      && (inFlight.Some? ==> inFlight.value.WF())
+    }
+
+    function Likes() : Likes {
+      if ephemeral.Known?
+      then ephemeral.v.ImperativeLikes()
+      else LikesJournal.TjTransitiveLikes(persistent)
+    }
+  } // end datatype Variables
+
+  
+  predicate LoadEphemeralFromPersistent(v: Variables, v': Variables, lbl: TransitionLabel)
+  {
+    && v.WF()
+    && lbl.base.LoadEphemeralFromPersistentLabel?
+    && lbl.allocs == []
+    && v.ephemeral.Unknown?
+    && v'.ephemeral.Known?
+
+    && LikesJournal.Init(v'.ephemeral.v, v.persistent)
+    && v'.persistent == v.persistent // UNCHANGED
+    && v'.inFlight == v.inFlight // UNCHANGED
+  }
+  
+  predicate ReadForRecovery(v: Variables, v': Variables, lbl: TransitionLabel)
+  {
+    && v.WF()
+    && lbl.base.ReadForRecoveryLabel?
+    && lbl.allocs == []
+    && v.ephemeral.Known?
+    && v'.ephemeral.Known?
+  
+    && LikesJournal.Next(v.ephemeral.v, v'.ephemeral.v, LikesJournal.ReadForRecoveryLabel(lbl.base.records))
+    && v' == v  // everything UNCHANGED
+  }
+
+  predicate QueryEndLsn(v: Variables, v': Variables, lbl: TransitionLabel)
+  {
+    && v.WF()
+    && lbl.base.QueryEndLsnLabel?
+    && lbl.allocs == []
+    && v.ephemeral.Known?
+    && v'.ephemeral.Known?
+
+    && LikesJournal.Next(v.ephemeral.v, v'.ephemeral.v, LikesJournal.QueryEndLsnLabel(lbl.base.endLsn))
+    && v' == v
+  }
+
+  predicate Put(v: Variables, v': Variables, lbl: TransitionLabel)
+  {
+    && v.WF()
+    && lbl.base.PutLabel?
+    && lbl.allocs == []
+    && v.ephemeral.Known?
+    && v'.ephemeral.Known?
+
+    && LikesJournal.Next(v.ephemeral.v, v'.ephemeral.v, LikesJournal.PutLabel(lbl.base.records))
+    && v'.persistent == v.persistent // UNCHANGED
+    && v'.inFlight == v.inFlight // UNCHANGED
+  }
+
+  predicate Internal(v: Variables, v': Variables, lbl: TransitionLabel)
+  {
+    && v.WF()
+    && lbl.base.InternalLabel?
+    && v.ephemeral.Known?
+    && v'.ephemeral.Known?
+
+    && LikesJournal.Next(v.ephemeral.v, v'.ephemeral.v, LikesJournal.InternalLabel(lbl.allocs))
+    && v'.persistent == v.persistent // UNCHANGED
+    && v'.inFlight == v.inFlight // UNCHANGED
+  }
+
+  predicate QueryLsnPersistence(v: Variables, v': Variables, lbl: TransitionLabel)
+  {
+    && v.WF()
+    && lbl.base.QueryLsnPersistenceLabel?
+    && lbl.allocs == []
+    && lbl.base.syncLsn <= v.persistent.SeqEnd()
+    && v' == v
+  }
+
+  predicate CommitStart(v: Variables, v': Variables, lbl: TransitionLabel)
+  {
+    && v.WF()
+    && lbl.base.CommitStartLabel?
+    && lbl.allocs == []
+    && v.ephemeral.Known?
+    // Can't start a commit if one is in-flight, or we'd forget to maintain the
+    // invariants for the in-flight one.
+    && v.inFlight.None?
+    && v'.ephemeral.Known?
+    && v'.inFlight.Some?
+
+    && var frozenJournal := v'.inFlight.value;
+
+    // Frozen journal stitches to frozen map
+    && frozenJournal.SeqStart() == lbl.base.newBoundaryLsn
+
+    // Journal doesn't go backwards
+    && frozenJournal.WF()
+    && v.persistent.SeqEnd() <= frozenJournal.SeqEnd()
+
+    // There should be no way for the frozen journal to have passed the ephemeral map!
+    && frozenJournal.SeqStart() <= lbl.base.maxLsn
+
+    && LikesJournal.Next(v.ephemeral.v, v'.ephemeral.v, LikesJournal.FreezeForCommitLabel(frozenJournal))
+
+    && v' == v.(
+      ephemeral := v'.ephemeral,  // given by predicate above (but happens to be read-only / unchanged)
+      inFlight := Some(frozenJournal) // given by predicates above
+      )
+  }
+
+  predicate CommitComplete(v: Variables, v': Variables, lbl: TransitionLabel)
+  {
+    && v.WF()
+    && lbl.base.CommitCompleteLabel?
+    && lbl.allocs == []
+    && v.ephemeral.Known?
+    && v.inFlight.Some?
+    && v'.ephemeral.Known?
+
+    && LikesJournal.Next(v.ephemeral.v, v'.ephemeral.v,
+        LikesJournal.DiscardOldLabel(v.inFlight.value.SeqStart(), lbl.base.requireEnd))
+
+    && v' == v.(
+      persistent := v.inFlight.value,
+      ephemeral := v'.ephemeral,  // given by predicate above
+      inFlight := None)
+  }
+
+  predicate Crash(v: Variables, v': Variables, lbl: TransitionLabel)
+  {
+    && v.WF()
+    && lbl.base.CrashLabel?
+    && lbl.allocs == []
+    && v' == v.(
+      ephemeral := Unknown,
+      inFlight := None)
+  }
+
+  // Models mkfs
+  predicate Init(v: Variables)
+  {
+    // TODO(tony): What is our default persistent here?
+    v == Variables(LikesJournal.EmptyJournalImage(), Unknown, None)
+  }
+
+  predicate Next(v: Variables, v': Variables, lbl: TransitionLabel)
+  {
+    match lbl.base {
+      case LoadEphemeralFromPersistentLabel() => LoadEphemeralFromPersistent(v, v', lbl)
+      case ReadForRecoveryLabel(_) => ReadForRecovery(v, v', lbl)
+      case QueryEndLsnLabel(_) => QueryEndLsn(v, v', lbl)
+      case PutLabel(_) => Put(v, v', lbl)
+      case InternalLabel() => Internal(v, v', lbl)
+      case QueryLsnPersistenceLabel(_) => QueryLsnPersistence(v, v', lbl)
+      case CommitStartLabel(_, _) => CommitStart(v, v', lbl)
+      case CommitCompleteLabel(_) => CommitComplete(v, v', lbl)
+      case CrashLabel() => Crash(v, v', lbl)
+    }
+  }
+
+
+} // end module LikesCrashTolerantJournal
